src/polytime/lemmas.lean
@@ -1,0 +1,159 @@
+import complexity_class.stack_rec
+import polytime.basic
+import polytime.stack_rec_size
+
+open tree (stack_step iterator_stack stack_step_polysize)
+open tencodable function polysize
+
+namespace polytime
+
+open_locale complexity_class
+
+variables {α β γ : Type} [tencodable α] [tencodable β] [tencodable γ]
+  [polysize α] [polysize β] [polysize γ]
+
+section stack_rec
+
+attribute [complexity] complexity_class.stack_iterate
+
+variables {base : γ → α → β} {pre₁ pre₂ : γ → tree unit → tree unit → α → α}
+  {post : γ → β → β → tree unit → tree unit → α → β}
+
+@[complexity]
+protected theorem stack_rec {st : γ -> tree unit} {arg : γ → α} (hst : st ∈ₑ PTIME) (harg : arg ∈ₑ PTIME) (hb : base ∈ₑ PTIME) (hpr₁ : pre₁ ∈ₑ PTIME) (hpr₂ : pre₂ ∈ₑ PTIME) (hpo : post ∈ₑ PTIME)
+  (hpr₁' : polysize_safe (λ (usf : γ × tree unit × tree unit) (sf : α), pre₁ usf.1 usf.2.1 usf.2.2 sf))
+  (hpr₂' : polysize_safe (λ (usf : γ × tree unit × tree unit) (sf : α), pre₂ usf.1 usf.2.1 usf.2.2 sf))
+  (hpo' : polysize_safe (λ (usf : γ × tree unit × tree unit × α) (sf : β × β), post usf.1 sf.1 sf.2 usf.2.1 usf.2.2.1 usf.2.2.2)) :
+  polytime.mem (λ x : γ, (st x).stack_rec (base x) (pre₁ x) (pre₂ x) (post x) (arg x)) :=
+begin
+  suffices : polytime.mem (λ x, (stack_step (base x) (pre₁ x) (pre₂ x) (post x))^[(st x).time_steps] [sum.inl (st x, arg x, none)]),
+  { rw complexity_class.of_some,
+    convert complexity_class.mem.comp (show polytime.mem (λ x : list (iterator_stack α β), x.head'.bind sum.get_right), by complexity) this, 
+    simp, },
+  apply iterate, { dsimp only [tree.time_steps], complexity, }, { complexity, }, { complexity, },
+  cases stack_step_polysize (polytime.size_le hst) (polytime.size_le harg)
+    (polytime.size_le hb) hpr₁' hpr₂' hpo' with p hp,
+  use p, intros x m _, exact hp x m,
+end
+
+lemma tree_eq : polytime.mem_pred (@eq (tree unit)) :=
+begin
+  rw ← complexity_class.mem_iff_mem_rel,
+  complexity using λ x y, x.stack_rec (λ y' : tree unit, (y' = tree.nil : bool))
+    (λ _ _ y', y'.left) (λ _ _ y', y'.right)
+    (λ b₁ b₂ _ _ y, !(y = tree.nil : bool) && (b₁ && b₂)) y,
+  { use 0, simpa using tree.left_num_nodes_le, }, { use 0, simpa using tree.right_num_nodes_le, }, { use 0, simp, },
+  induction x using tree.unit_rec_on with l r ih₁ ih₂ generalizing y; cases y; simp [*],
+end
+
+@[complexity] lemma eq : (@eq α) ∈ₚ PTIME :=
+by { have := tree_eq, complexity using (λ x y, encode x = encode y), simp, }
+
+end stack_rec
+
+section list
+
+@[complexity] lemma list_len : (@list.length α) ∈ₑ PTIME :=
+begin
+  complexity using λ x, (encode x).stack_rec (λ _ : unit, 0) (λ _ _ _, ()) (λ _ _ _, ())
+    (λ _ ih _ _ _, ih + 1) (),
+  { use 0, simp, }, { use 0, simp, }, { use 1, simp, },
+  induction x with hd tl ih, { refl, },
+  simpa [encode_cons],
+end
+
+@[simp] def scanl_step {α β : Type*} (f : β → α → β) : list α × list β → list α × list β
+| ((x :: xs), (y :: ys)) := (xs, f y x :: y :: ys)
+| x := x
+
+@[complexity] theorem scanl_step_polytime {f : γ → β → α → β} {st : γ → list α × list β} (hf : f ∈ₑ PTIME) (hst : st ∈ₑ PTIME) :
+  (λ x, scanl_step (f x) (st x)) ∈ₑ PTIME :=
+by { delta scanl_step, clean_target, complexity, }
+
+theorem scanl_step_iterate' {α : Type*} (f : β → α → β) (l : list α) (x : β) (n : ℕ) :
+  (scanl_step f)^[n] (l, [x]) = (l.drop n, ((l.scanl f x).take (n + 1)).reverse) :=
+begin
+  suffices : ∀ xs, (scanl_step f)^[n] (l, x :: xs) = (l.drop n, ((l.scanl f x).take (n + 1)).reverse ++ xs),
+  { simpa using this [], },
+  intro xs,
+  induction l with hd tl ih generalizing x xs n, { rw iterate_fixed; simp, },
+  cases n, { simp, }, { simp [ih], },
+end
+
+theorem scanl_step_iterate {α : Type*} (f : β → α → β) (l : list α) (x : β) :
+  (scanl_step f)^[l.length] (l, [x]) = ([], (l.scanl f x).reverse) :=
+by { rw [scanl_step_iterate', ← @list.length_scanl _ _ f x l], simp, }
+
+theorem foldl_size_le (f : β → α → β) (p : ℕ → ℕ) (hp : monotone p)
+  (hf : ∀ x y, size (f x y) ≤ size x + p (size y)) (ls : list α) (x₀ : β) :
+  size (ls.foldl f x₀) ≤ size x₀ + ls.length * p (size ls) :=
+begin
+  induction ls with hd tl ih generalizing x₀, { simp, },
+  rw [list.foldl, list.length_cons, nat.succ_mul, ← add_assoc, add_right_comm],
+  refine (ih _).trans (add_le_add ((hf _ _).trans $ add_le_add_left (hp _) _) (mul_le_mul_left' (hp _) _));
+  simp; linarith only,
+end
+
+lemma list_scanl_rev {lst : γ → list α} {acc : γ → β} {f : γ → β → α → β}
+  (hlst : lst ∈ₑ PTIME) (hacc : acc ∈ₑ PTIME) (hf : f ∈ₑ PTIME)
+  (hf' : polysize_safe (λ (usf : γ × α) (sf : β), f usf.1 sf usf.2)) :
+  polytime.mem (λ x : γ, ((lst x).scanl (f x) (acc x)).reverse) :=
+begin
+  convert_to polytime.mem (λ x, ((scanl_step (f x))^[(lst x).length] (lst x, [acc x])).2),
+  { simp [scanl_step_iterate], },
+  refine complexity_class.mem.snd.comp _,
+  apply iterate,
+  { complexity, }, { complexity, }, { complexity, },
+  cases hf' with pf hpf, cases polytime.size_le hlst with pl hpl, cases polytime.size_le hacc with pa hpa,
+  use pl + (pl + 1) * (pa + pl * pf.comp (polynomial.X + pl) + 1),
+  intros x m _,
+  simp [scanl_step_iterate'], apply add_le_add,
+  { exact (list.size_le_of_sublist ((lst x).drop_sublist _)).trans (hpl _), },
+  refine (list.size_le_of_sublist (list.take_sublist _ _)).trans _,
+  apply list.size_le_mul_of_le,
+  { rw [list.length_scanl, add_le_add_iff_right], exact (lst x).length_le_size.trans (hpl _), },
+  simp_rw list.mem_iff_nth_le,
+  rintros e ⟨n, hn, rfl⟩,
+  rw list.scanl_nth_le_eq_foldl,
+  refine (foldl_size_le (f x) (λ a, pf.eval (size (x, a))) (λ a b h, pf.eval_mono $ add_le_add_left h _) (λ b a, hpf (x, a) b) _ _).trans _,
+  simp, mono*,
+  { exact min_le_of_right_le ((lst x).length_le_size.trans (hpl _)), },
+  { exact (list.size_le_of_sublist (list.take_sublist _ _)).trans (hpl _), },
+  exacts [zero_le', zero_le'],
+end
+
+@[complexity] lemma list_foldl {lst : γ → list α} {acc : γ → β} {f : γ → β → α → β}
+  (hlst : lst ∈ₑ PTIME) (hacc : acc ∈ₑ PTIME) (hf : f ∈ₑ PTIME)
+  (hf' : polysize_safe (λ (usf : γ × α) (sf : β), f usf.1 sf usf.2)) :
+  polytime.mem (λ x : γ, (lst x).foldl (f x) (acc x)) :=
+begin
+  rw complexity_class.of_some,
+  convert complexity_class.head'.comp (list_scanl_rev hlst hacc hf hf'),
+  ext x : 1, simp [list.scanl_last_eq_foldl],
+end
+
+@[complexity] theorem list_reverse : (@list.reverse α) ∈ₑ PTIME :=
+begin
+  complexity using (λ l : list α, l.foldl (λ (acc : list α) (hd : α), hd :: acc) []),
+  rw [← list.foldr_reverse, list.foldr_eta],
+end
+
+@[complexity] lemma list_scanl {lst : γ → list α} {acc : γ → β} {f : γ → β → α → β}
+  (hlst : lst ∈ₑ PTIME) (hacc : acc ∈ₑ PTIME) (hf : f ∈ₑ PTIME)
+  (hf' : polysize_safe (λ (usf : γ × α) (sf : β), f usf.1 sf usf.2)) :
+  polytime.mem (λ x : γ, ((lst x).scanl (f x) (acc x))) :=
+by simpa using list_reverse.comp (list_scanl_rev hlst hacc hf hf')
+
+@[complexity] theorem list_foldr {lst : γ → list α} {acc : γ → β} {f : γ → α → β → β}
+  (hlst : lst ∈ₑ PTIME) (hacc : acc ∈ₑ PTIME) (hf : f ∈ₑ PTIME)
+  (hf' : polysize_safe (λ (usf : γ × α) (sf : β), f usf.1 usf.2 sf)) :
+  polytime.mem (λ x : γ, (lst x).foldr (f x) (acc x)) :=
+by { simp_rw ← list.foldl_reverse, complexity, }
+
+@[complexity] theorem list_map {lst : γ → list α} {f : γ → α → β} (hlst : lst ∈ₑ PTIME) (hf : f ∈ₑ PTIME) :
+  polytime.mem (λ x, (lst x).map (f x)) :=
+by { complexity using (λ x, (lst x).foldr (λ hd acc, (f x hd) :: acc) []), induction lst x; simp [*], }
+
+end list
+
+end polytime
